Clear/Utilities.lean
@@ -82,4 +82,31 @@ lemma evm_eq_symm_of_isPure_ok_ok {evm evm'} {vs vs'} (h : isPure (Ok evm vs) (O
   symm
   aesop_spec
 
+def preservesEvm (s₀ : State) (s₁ : State) : Prop :=
+  match s₀, s₁ with
+  | .Ok e₀ _, .Ok e₁ _ => preserved e₀ e₁
+  | _, _ => True
+
+@[simp]
+lemma preservesEvm_rfl {s : State} : preservesEvm s s := by
+  unfold preservesEvm
+  cases s <;> simp
+
+@[simp]
+lemma preservesEvm_trans {s₀ s₁ s₂} (h : s₁.isOk) :
+  preservesEvm s₀ s₁ → preservesEvm s₁ s₂ → preservesEvm s₀ s₂ := by
+  unfold preservesEvm
+  cases s₀ <;> cases s₁ <;> cases s₂ <;> simp_all
+  exact preserved_trans
+
+lemma sload_eq_of_preservesEvm
+  {s s' : State} {a : UInt256} (h : s.isOk) (h' : s'.isOk) (hss : preservesEvm s s') :
+  s.evm.sload a = s'.evm.sload a := by
+  cases s <;> cases s' <;> simp_all
+  simp only [evm]
+  unfold EVMState.sload EVMState.lookupAccount
+  rw [ preserves_account_map hss
+     , preserves_execution_env hss
+     ]
+
 end Clear.Utilities
